\section{Theory}

\lipsum[30]

\nopagebreak

\begin{strip}
\begin{equation}
\begin{aligned}
\sum \vect{F} = m\vect{a} &= \vect{F}_{\text{restoring}} + \vect{F}_{\text{damping}} \\
                m\vect{g} &= -k\vect{x} - b\vect{v} \\
                        0 &= k\vect{x} + b\odv{\vect{x}}{t} + m\odv[2]{\vect{x}}{t} \\
                        0 &= k\vect{x} + b\odv{\vect{x}}{t} + m\odv[2]{\vect{x}}{t} \\
						0 &= \frac{k}{m}\vect{x} + \frac{b}{m}\odv{\vect{x}}{t} + \odv[2]{\vect{x}}{t} \\
						0 &= \frac{k}{m}e^{ut} + \frac{b}{m}\odv{(e^{ut})}{t} + \odv[2]{(e^{ut})}{t} \\
						0 &= k + bu + mu^2 \\
						u &= \frac{-b \pm \sqrt{b^2 - 4km}}{2m}
\end{aligned}
\end{equation}

\vspace{0.5em}
\begin{center}
\text{Assume the spring is underdamped (\textit{i.e.} $b^2 - 4km < 0$)}
\end{center}

\begin{equation}
\begin{aligned}
\vect{x} &= \alpha e^{\left(\frac{-b + \sqrt{b^2 - 4km}}{2m}\right)t} + \beta e^{\left(\frac{-b - \sqrt{b^2 - 4km}}{2m}\right)t} \\
		 &= e^{-\tfrac{bt}{2m}}\left[ \alpha e^{\left(\frac{\sqrt{b^2 - 4km}}{2m}\right)t} + \beta e^{\left(\frac{-\sqrt{b^2 - 4km}}{2m}\right)t} \right] \\
         &= e^{-\tfrac{bt}{2m}}\left[ \alpha e^{\left(\tfrac{i\sqrt{4km - b^2}}{2m}\right)t} + \beta e^{\left(\tfrac{-i\sqrt{4km - b^2}}{2m}\right)t} \right] \\
         &= e^{-\tfrac{bt}{2m}}\left[ (\alpha+\beta)\cos\left(\tfrac{\sqrt{4km - b^2}}{2m}t\right) + i(\alpha-\beta)\sin\left(\frac{t\sqrt{4km - b^2}}{2m}t\right)\right] \\
	     &= 2\sqrt{\alpha\beta}e^{\left(-\tfrac{b}{2m}\right)t}\cos\left(\tfrac{\sqrt{4km - b^2}}{2m}t + \phi\right)
\end{aligned}
\end{equation}

\vspace{2em}
\begin{equation*}
\begin{aligned}
\text{Let } A &= 2\sqrt{\alpha\beta} \\
       \gamma &= \frac{b}{2m} \\
      \omega' &= \frac{\sqrt{4km - b^2}}{2m}
\end{aligned}
\end{equation*}

\vspace{1em}
\begin{equation} 
\therefore \vect{x} = Ae^{-\gamma t} \cos\left(\omega' t + \phi\right)
\end{equation}
\end{strip}

\lipsum[31-32]
\begin{equation}
\begin{aligned}
             \omega' &= \frac{\sqrt{4 k m - b^2}}{2 m} \\
           \omega'^2 &= \frac{4 k m - b^2}{4 m^2} \\
           \omega'^2 &= \frac{k}{m} - \frac{b^2}{4 m^2} \\
           \omega'^2 &= \frac{k}{m} - \gamma^2 \quad \quad \text{with } \gamma = \frac{b}{2 m} \\
\omega'^2 + \gamma^2 &= k \left(\frac{1}{m}\right)
\end{aligned}
\end{equation}

\lipsum[33]