\section{Evaluation}

\lipsum[10]

\begin{align*}
\intertext{Let $m_{\mathrm{eq}} = m_{\mathrm{load}} + \tfrac{1}{3} m_{\mathrm{spring}}$ and $\lambda = m_{\mathrm{load}}^{-1}$}
\gamma &= \frac{b}{2 m_{\mathrm{eq}}} \\
       &= \frac{b}{2 \left(m_{\mathrm{load}} + \tfrac{1}{3} m_{\mathrm{spring}}\right)} \\
       &= \frac{b}{2 \left(\tfrac{1}{\lambda} + \tfrac{1}{3} m_{\mathrm{spring}}\right)} \\
       &= \frac{b}{2} \frac{\lambda}{1 + \tfrac{1}{3} m_{\mathrm{spring}} \, \lambda} \\
\therefore \frac{d \gamma}{d \lambda} &= \frac{b}{2} \frac{1}{\left(1 + \tfrac{1}{3} m_{\mathrm{spring}} \, \lambda\right)^2}
\end{align*}

\vspace{1em}

\lipsum[11 - 13]